proof/list_trivial_proof.v
@@ -243,12 +243,82 @@ Proof.
   vauto.
 Qed.
 
+
+Lemma above_doc_app (fs l1 l2 : list t) (w : Z):
+  FormatTrivial.aboveDoc (Z.to_nat w) fs l1 ++
+    FormatTrivial.aboveDoc (Z.to_nat w) fs l2 =
+      FormatTrivial.aboveDoc (Z.to_nat w) fs (l1 ++ l2).
+Proof.
+  unfold FormatTrivial.aboveDoc.
+  unfold FormatTrivial.cross_general.
+  rewrite <- filter_app.
+  rewrite <- concat_app.
+  rewrite <- map_app.
+  vauto.
+Qed.
+
+Lemma fill_doc_app (fs l1 l2 : list t) (w shift : Z):
+  FormatTrivial.fillDoc (Z.to_nat w) fs l1 (Z.to_nat shift) ++
+    FormatTrivial.fillDoc (Z.to_nat w) fs l2 (Z.to_nat shift) =
+      FormatTrivial.fillDoc (Z.to_nat w) fs (l1 ++ l2) (Z.to_nat shift).
+Proof.
+  unfold FormatTrivial.fillDoc.
+  unfold FormatTrivial.cross_general.
+  rewrite <- filter_app.
+  rewrite <- concat_app.
+  rewrite <- map_app.
+  vauto.
+Qed.
+
+
 Lemma beside_doc_app_l (l1 l2: list t) (w : Z) (G : t):
   FormatTrivial.besideDoc (Z.to_nat w) l1 [G] ++
     FormatTrivial.besideDoc (Z.to_nat w) l2 [G] =
       FormatTrivial.besideDoc (Z.to_nat w) (l1 ++ l2) [G].
 Proof.
   unfold FormatTrivial.besideDoc.
+  unfold FormatTrivial.cross_general.
+  repeat rewrite <- filter_app.
+  repeat rewrite <- concat_app.
+  repeat rewrite map_cons.
+  repeat rewrite map_nil.
+  repeat rewrite concat_app.
+  repeat rewrite concat_cons.
+  repeat rewrite concat_nil.
+  autorewrite with sublist norm.
+  repeat rewrite filter_app.
+  repeat rewrite map_app.
+  repeat rewrite filter_app.
+  vauto.
+Qed.
+
+Lemma above_doc_app_l (l1 l2: list t) (w : Z) (G : t):
+  FormatTrivial.aboveDoc (Z.to_nat w) l1 [G] ++
+    FormatTrivial.aboveDoc (Z.to_nat w) l2 [G] =
+      FormatTrivial.aboveDoc (Z.to_nat w) (l1 ++ l2) [G].
+Proof.
+  unfold FormatTrivial.aboveDoc.
+  unfold FormatTrivial.cross_general.
+  repeat rewrite <- filter_app.
+  repeat rewrite <- concat_app.
+  repeat rewrite map_cons.
+  repeat rewrite map_nil.
+  repeat rewrite concat_app.
+  repeat rewrite concat_cons.
+  repeat rewrite concat_nil.
+  autorewrite with sublist norm.
+  repeat rewrite filter_app.
+  repeat rewrite map_app.
+  repeat rewrite filter_app.
+  vauto.
+Qed.
+
+Lemma fill_doc_app_l (l1 l2: list t) (w shift : Z) (G : t):
+  FormatTrivial.fillDoc (Z.to_nat w) l1 [G] (Z.to_nat shift) ++
+    FormatTrivial.fillDoc (Z.to_nat w) l2 [G] (Z.to_nat shift) =
+      FormatTrivial.fillDoc (Z.to_nat w) (l1 ++ l2) [G] (Z.to_nat shift).
+Proof.
+  unfold FormatTrivial.fillDoc.
   unfold FormatTrivial.cross_general.
   repeat rewrite <- filter_app.
   repeat rewrite <- concat_app.
@@ -614,7 +684,6 @@ Proof.
   rewrite (filter_good_format (fs1 ++ fs2) w h); vauto.
   apply good_format_app; vauto.
 Qed.
-
 
 Lemma body_beside_doc : semax_body Vprog Gprog f_beside_doc beside_doc_spec.
 Proof.
@@ -1295,5 +1364,1353 @@ desf;
 assert (
   (total_width (add_beside (Znth j fs1) (Znth i fs2)) <= Z.to_nat w)%nat /\
     (height (add_beside (Znth j fs1) (Znth i fs2)) <= Z.to_nat h)%nat
+) as GG by auto; desf.
+Qed.
+
+Lemma body_fill_doc : semax_body Vprog Gprog f_fill_doc fill_doc_spec.
+Proof.
+  start_function.
+  forward_if(p1 <> nullval).
+  { forward_if(
+    PROP ( )
+    LOCAL (gvars gv; temp _shift (Vptrofs (Ptrofs.repr shift)); temp _width (Vint (Int.repr w)); temp _height (Vint (Int.repr h)); temp _fs1 p1; temp _fs2 p2)
+    SEP (listrepf fs1 p1 w h; mem_mgr gv)).
+    { forward_call(fs2, p2, w, h, gv); entailer!. }
+    { forward; entailer!. 
+      unnw; desf.
+      assert (fs2 = []) by auto; subst.
+      unff listrepf; entailer!. }
+    forward.
+    unnw; desf.
+    assert (fs1 = []) by auto; subst.
+    Exists nullval ([] : list t); entailer!.
+    unfold FormatTrivial.fillDoc.
+    unfold FormatTrivial.cross_general; ins.
+    rewrite concat_map_nil; list_solve. }
+  { forward; entailer!. }
+
+  forward_if(p2 <> nullval).
+  { forward_call(fs1, p1, w, h, gv).
+    forward.
+    unnw; desf.
+    assert (fs2 = []) by auto; subst.
+    Exists nullval ([] : list t); entailer!. }
+  { forward; entailer!. }
+  forward_call(t_flist, gv).
+  Intros result_ptr.
+  dest_ptr result_ptr.
+  forward_call(gv).
+  Intros cur_empty_ptr.
+  do 3 forward.
+  desf.
+  do 2 forward.
+  
+
+  remember (
+      EX i : Z, EX head_ptr : val, EX result_tail_ptr : val, EX res_part : list t,
+      PROP(0 <= i <= Zlength fs2;
+            res_part = filter (fun G => (G.(height) <=? Z.to_nat h)%nat) (FormatTrivial.fillDoc (Z.to_nat w) fs1 (sublist 0 i fs2) (Z.to_nat shift)))
+      LOCAL(temp _fs2_tail head_ptr;
+            temp _shift (Vptrofs (Ptrofs.repr shift));
+            temp _has_item (Val.of_bool (0 <? Zlength res_part)); temp _result result_ptr; gvars gv; 
+            temp _width (Vint (Int.repr w)); temp _height (Vint (Int.repr h));
+            temp _fs1 p1; temp _fs2 p2; temp _result_tail result_tail_ptr)
+      SEP (mem_mgr gv; listrepf fs1 p1 w h; lsegf (sublist 0 i fs2) p2 head_ptr w h; 
+          listrepf (sublist i (Zlength fs2) fs2) head_ptr w h; lsegf res_part result_ptr result_tail_ptr w h;
+          listrepf [empty] result_tail_ptr w h)) as loop_invariant eqn:eqn_loop.
+  remember (
+      EX result_tail_ptr : val, EX res_part : list t,
+      PROP(res_part = filter (fun G => (G.(height) <=? Z.to_nat h)%nat) (FormatTrivial.fillDoc (Z.to_nat w) fs1 fs2 (Z.to_nat shift)))
+      LOCAL(temp _has_item (Val.of_bool (0 <? Zlength res_part)); temp _result result_ptr; gvars gv;
+            temp _result_tail result_tail_ptr;
+            temp _shift (Vptrofs (Ptrofs.repr shift));
+            temp _width (Vint (Int.repr w)); temp _height (Vint (Int.repr h));
+            temp _fs1 p1; temp _fs2 p2)
+      SEP (mem_mgr gv; listrepf fs1 p1 w h; listrepf fs2 p2 w h; lsegf res_part result_ptr result_tail_ptr w h;
+          listrepf [empty] result_tail_ptr w h)) as break_invariant eqn:eqn_break.
+  forward_loop(loop_invariant) break: (break_invariant).
+  { subst.
+    Exists 0 p2 result_ptr ([] : list t).
+    entailer!.
+    replace (sublist 0 0 fs2) with ([] : list t) by list_solve.
+    assert (sublist 0 (Zlength fs2) fs2 = fs2) as K.
+    { rewrite sublist_skip; vauto. }
+    rewrite K.
+    unff lsegf; entailer!; ins.
+    unfold mformat.
+    Intros sigma_list sigma_pt.
+    unff listrepf.
+    Exists nullval cur_empty_ptr sigma_list sigma_pt.
+    unfold concrete_mformat.
+    entailer!.
+    getnw.
+    inv FMT_MP.
+    unfold empty in *; ins.
+    unnw; unfold good_format; ins.
+    assert (sigma_list = []) by list_solve; subst.
+    list_solve. }
+  2: { subst.
+      Intros result_tail_ptr res_part.
+      forward_call(fs1, p1, w, h, gv).
+      forward_call(fs2, p2, w, h, gv).
+      forward_if (
+        Zlength res_part <> 0
+      ).
+      { destruct (0 <? Zlength res_part) eqn:E; vauto.
+        forward_call([empty], result_ptr, w, h, gv).
+        { desf; entailer!.
+          replace ((filter (fun G : t => (height G <=? Z.to_nat h)%nat)
+          (FormatTrivial.fillDoc (Z.to_nat w) fs1 fs2 (Z.to_nat shift)))) with ([] : list t) by list_solve.
+          unff lsegf; unff listrepf.
+          entailer!; subst; unnw; entailer!.
+          Exists nullval y format_sigma sigma_pt; entailer!. }
+        forward.
+        Exists nullval ([] : list t); entailer!.
+        2: { unff listrepf; entailer!. }
+        list_solve. }
+      { forward; entailer!; ins.
+        assert (Zlength (filter (fun G : t => (height G <=? Z.to_nat h)%nat)
+           (FormatTrivial.fillDoc (Z.to_nat w) fs1 fs2 (Z.to_nat shift))) = 0) as K by vauto.
+        rewrite K in *; vauto. }
+      forward.
+      forward_loop(
+        EX i : Z, EX new_result_tail : val,
+        PROP(0 <= i < Zlength res_part)
+        LOCAL(temp _new_result_tail new_result_tail; temp _fs1 p1; temp _fs2 p2; 
+              temp _result_tail result_tail_ptr; gvars gv; temp _result result_ptr)
+        SEP(mem_mgr gv; lsegf (sublist 0 i res_part) result_ptr new_result_tail w h; 
+            listrepf (sublist i (Zlength res_part) res_part ++ [empty]) new_result_tail w h)
+      ) break: (
+        EX new_result_tail : val,
+        PROP()
+        LOCAL(temp _new_result_tail new_result_tail; temp _fs1 p1; temp _fs2 p2; 
+              temp _result_tail result_tail_ptr; gvars gv; temp _result result_ptr)
+        SEP(mem_mgr gv; lsegf (sublist 0 (Zlength res_part - 1) res_part) result_ptr new_result_tail w h; 
+            listrepf (sublist (Zlength res_part - 1) (Zlength res_part) res_part ++ [empty]) new_result_tail w h)).
+      { Exists 0 result_ptr.
+        entailer!.
+        autorewrite with sublist.
+        unff lsegf; entailer!.
+        apply lsegf_listf. }
+      { Intros i new_result_tail_ptr.
+        replace (sublist i (Zlength res_part) res_part) with (Znth i res_part :: sublist (i + 1) (Zlength res_part) res_part)
+          by list_solve.
+        autorewrite with sublist norm.
+        replace ((Znth i res_part
+            :: sublist (i + 1) (Zlength res_part) res_part) ++ [empty]) with
+            (Znth i res_part :: (sublist (i + 1) (Zlength res_part) res_part ++ [empty])) by list_solve.
+        unff listrepf.
+        Intros ith_tail_ptr ith_format_ptr format_sigma sigma_pt.
+        forward.
+        { entailer!; getnw; desf. }
+        assert (i + 1 = Zlength res_part \/ i + 1 < Zlength res_part) as K by lia.
+        destruct K.
+        { replace (sublist (i + 1) (Zlength res_part) res_part) with ([] : list t) by list_solve.
+          autorewrite with sublist.
+          unff listrepf.
+          Intros nullval_tail_ptr empty_ptr format_sigma_empty sigma_pt_empty.
+          forward.
+          { unnw; subst; entailer!. }
+          getnw; rewrite LIST_NULL_PTR.
+          forward_if.
+          { vauto. }
+          forward.  
+          entailer!.
+          Exists new_result_tail_ptr.
+          remember (filter (fun G : t => (height G <=? Z.to_nat h)%nat) (FormatTrivial.fillDoc (Z.to_nat w) fs1 fs2 (Z.to_nat shift)))
+            as res_part.
+          replace i with (Zlength res_part - 1) by lia.
+          replace (sublist (Zlength res_part - 1) (Zlength res_part) res_part ++ [empty])
+            with [Znth (Zlength res_part - 1) res_part; empty] by list_solve.
+          unff listrepf.
+          Exists ith_tail_ptr ith_format_ptr format_sigma sigma_pt.
+          Exists nullval empty_ptr format_sigma_empty sigma_pt_empty.
+          entailer!.
+          unnw.
+          list_solve. }
+        replace (sublist (i + 1) (Zlength res_part) res_part)
+          with (Znth (i + 1) res_part :: sublist (i + 2) (Zlength res_part) res_part) by list_solve.
+        replace ((Znth (i + 1) res_part :: sublist (i + 2) (Zlength res_part) res_part) ++ [empty]) with
+            (Znth (i + 1) res_part :: ((sublist (i + 2) (Zlength res_part) res_part ++ [empty]))) by list_solve.
+        unff listrepf.
+        Intros ithplus_tail_ptr ithplus_format_ptr ith_plus_sigma ith_plus_sigma_pt.
+        forward.
+        { entailer!; unnw; desf.  }
+        forward_if.
+        { forward; entailer!.
+          remember (filter (fun G : t => (height G <=? Z.to_nat h)%nat) (FormatTrivial.fillDoc (Z.to_nat w) fs1 fs2 (Z.to_nat shift))).
+          Exists (i + 1) ith_tail_ptr.
+          replace (sublist (i + 1) (Zlength l) l) with
+              (Znth (i + 1) l :: sublist (i + 2) (Zlength l) l) by list_solve.
+          replace ((Znth (i + 1) l :: sublist (i + 2) (Zlength l) l) ++ [empty]) with 
+              (Znth (i + 1) l :: (sublist (i + 2) (Zlength l) l ++ [empty])) by list_solve.
+          unff listrepf.
+          Exists ithplus_tail_ptr ithplus_format_ptr ith_plus_sigma ith_plus_sigma_pt.
+          entailer!.
+          remember (filter (fun G : t => (height G <=? Z.to_nat h)%nat) (FormatTrivial.fillDoc (Z.to_nat w) fs1 fs2 (Z.to_nat shift))).
+          assert (
+            lsegf (sublist 0 i l) result_ptr new_result_tail_ptr w h *
+            lsegf [Znth i l] new_result_tail_ptr ith_tail_ptr w h |--
+            lsegf (sublist 0 (i + 1) l) result_ptr ith_tail_ptr w h) as K.
+          { replace (sublist 0 (i + 1) l) with (sublist 0 i l ++ [Znth i l]) by list_solve.
+            eapply lsegf_lsegf. }
+          eapply derives_trans.
+          2: eauto.
+          entailer!.
+          unff lsegf; Exists ith_tail_ptr ith_format_ptr format_sigma sigma_pt.
+          entailer!. }
+        forward.
+        replace ithplus_tail_ptr with nullval by vauto.
+        destruct (sublist (i + 2) (Zlength res_part) res_part).
+        { autorewrite with sublist norm.
+          unff listrepf.
+          Intros x y format_sigma0 sigma_pt0.
+          entailer!. }
+        replace (((t :: l) ++ [empty])) with (t :: (l ++ [empty])) by list_solve.
+        unff listrepf.
+        Intros x y format_sigma0 sigma_pt0.
+        entailer!. }
+    Intros new_result_tail.
+    replace (sublist (Zlength res_part - 1) (Zlength res_part) res_part ++ [empty]) with 
+        [Znth (Zlength res_part - 1) res_part; empty] by list_solve.
+    unff listrepf.
+    Intros empty_list_ptr last_format_ptr empty_sigma empty_sigma_ptr.
+    Intros nullval_ptr empty_format_ptr format_sigma0 sigma_pt0.
+    forward.
+    forward_call([empty], empty_list_ptr, w, h, gv).
+    { getnw; subst.
+      unff listrepf.
+      Exists nullval empty_format_ptr format_sigma0 sigma_pt0.
+      entailer!. }
+    do 2 forward.
+    Exists result_ptr (filter (fun G : t => (height G <=? Z.to_nat h)%nat) (FormatTrivial.fillDoc (Z.to_nat w) fs1 fs2 (Z.to_nat shift))).
+    entailer!.
+    remember (filter (fun G : t => (height G <=? Z.to_nat h)%nat) (FormatTrivial.fillDoc (Z.to_nat w) fs1 fs2 (Z.to_nat shift))).
+    assert (
+      lsegf (sublist 0 (Zlength l - 1) l) result_ptr new_result_tail w h *
+      listrepf [Znth (Zlength l - 1) l] new_result_tail w h |--
+      listrepf l result_ptr w h
+    ) as K.
+    { assert(l = (sublist 0 (Zlength l - 1) l ++ [Znth (Zlength l - 1) l])) as KK by list_solve.
+      rewrite KK at 5.
+      apply lsegf_listf. }
+    eapply derives_trans.
+    2: eauto.
+    unff listrepf.
+    Exists nullval last_format_ptr empty_sigma empty_sigma_ptr.
+    entailer!. }
+subst.
+Intros i head_ptr result_tail_ptr res_part.
+forward_if.
+2: {
+  forward.
+  Exists result_tail_ptr res_part.
+  assert(i < Zlength fs2 \/ i = Zlength fs2) as K by lia.
+  destruct K.
+  { replace (sublist i (Zlength fs2) fs2) with 
+      (Znth i fs2 :: sublist (i + 1) (Zlength fs2) fs2) by list_solve.
+    unff listrepf.
+    Intros x1 y1 x2 y2.
+    subst.
+    entailer!. }
+  entailer!.
+  { autorewrite with sublist norm; vauto. }
+  autorewrite with sublist norm.
+  unff listrepf.
+  entailer!.
+  apply lsegf_null_listrepf. }
+forward.
+remember (
+    EX j : Z, EX head_ptr2 : val, EX result_tail_ptr_new : val, EX res_part_new : list t,
+    PROP(0 <= j <= Zlength fs1;
+          res_part_new = res_part ++ filter (fun G => (G.(height) <=? Z.to_nat h)%nat) (FormatTrivial.fillDoc (Z.to_nat w) (sublist 0 j fs1) [Znth i fs2] (Z.to_nat shift)))
+    LOCAL(temp _fs2_tail head_ptr; temp _fs1_tail head_ptr2;
+          temp _has_item (Val.of_bool (0 <? Zlength res_part_new)); 
+          temp _shift (Vptrofs (Ptrofs.repr shift));
+          temp _result result_ptr; gvars gv; 
+          temp _width (Vint (Int.repr w)); temp _height (Vint (Int.repr h));
+          temp _fs1 p1; temp _fs2 p2; temp _result_tail result_tail_ptr_new)
+    SEP (mem_mgr gv; 
+        lsegf (sublist 0 j fs1) p1 head_ptr2 w h;
+        listrepf (sublist j (Zlength fs1) fs1) head_ptr2 w h;
+        lsegf (sublist 0 i fs2) p2 head_ptr w h; 
+        listrepf (sublist i (Zlength fs2) fs2) head_ptr w h; 
+        lsegf res_part_new result_ptr result_tail_ptr_new w h;
+        listrepf [empty] result_tail_ptr_new w h)) as loop_invariant eqn:eqn_loop.
+remember (
+    EX result_tail_ptr_new : val, EX res_part_new : list t,
+    PROP(res_part_new = filter (fun G => (G.(height) <=? Z.to_nat h)%nat) (FormatTrivial.fillDoc (Z.to_nat w) fs1 (sublist 0 (i + 1) fs2 ) (Z.to_nat shift)))
+    LOCAL(temp _has_item (Val.of_bool (0 <? Zlength res_part_new)); 
+          temp _result result_ptr; 
+          gvars gv;
+          temp _shift (Vptrofs (Ptrofs.repr shift));
+          temp _result_tail result_tail_ptr_new;
+          temp _width (Vint (Int.repr w)); temp _height (Vint (Int.repr h));
+          temp _fs1 p1; temp _fs2 p2;
+          temp _fs2_tail head_ptr)
+    SEP (mem_mgr gv; 
+        listrepf fs1 p1 w h; 
+        lsegf (sublist 0 i fs2) p2 head_ptr w h; 
+        listrepf (sublist i (Zlength fs2) fs2) head_ptr w h; 
+        lsegf res_part_new result_ptr result_tail_ptr_new w h;
+        listrepf [empty] result_tail_ptr_new w h)) as break_invariant eqn:eqn_break.
+forward_loop(loop_invariant) break: (break_invariant).
+{ rewrite eqn_loop.
+  Exists 0 p1 result_tail_ptr res_part.
+  entailer!.
+  { autorewrite with sublist norm; vauto. }
+  autorewrite with sublist norm.
+  unff lsegf; entailer!. }
+2: {
+  rewrite eqn_break.
+  Intros result_tail_ptr_new res_part_new.
+  assert(i = Zlength fs2 \/ i < Zlength fs2) as K by lia.
+  destruct K.
+  { subst.
+    autorewrite with sublist norm.
+    unff listrepf.
+    Intros; unnw; vauto. }
+  replace (sublist i (Zlength fs2) fs2) 
+    with (Znth i fs2 :: (sublist (i + 1) (Zlength fs2) fs2)) by list_solve.
+  unff listrepf.
+  Intros ith_tail_ptr ith_format_ptr ith_sigma ith_sigma_pt.
+  Intros nullval_ptr empty_ptr empty_sigma empty_sigma_pt.
+  getnw; rewrite LIST_NULL_PTR.
+  forward.
+  { entailer!; unnw; desf. }
+  Exists (i + 1) ith_tail_ptr result_tail_ptr_new res_part_new.
+  entailer!.
+  unff listrepf.
+  Exists nullval empty_ptr empty_sigma empty_sigma_pt.
+  entailer!.
+  assert (
+    lsegf (sublist 0 i fs2) p2 head_ptr w h *
+    lsegf [Znth i fs2] head_ptr ith_tail_ptr w h |--
+    lsegf (sublist 0 (i + 1) fs2) p2 ith_tail_ptr w h
+  ) as K.
+  { replace (sublist 0 (i + 1) fs2) with
+      (sublist 0 i fs2 ++ [Znth i fs2]) by list_solve.
+    apply lsegf_lsegf. }
+  eapply derives_trans.
+  2: eauto.
+  entailer!.
+  unff lsegf; entailer!.
+  Exists ith_tail_ptr ith_format_ptr ith_sigma ith_sigma_pt.
+  entailer!. }
+rewrite eqn_loop.
+Intros j head_ptr2 result_tail_ptr_new res_part_new.
+forward_if.
+2: { 
+  forward.
+  rewrite eqn_break.
+  Exists result_tail_ptr_new 
+    (filter (fun G : t => (height G <=? Z.to_nat h)%nat) (FormatTrivial.fillDoc (Z.to_nat w) fs1 (sublist 0 (i + 1) fs2) (Z.to_nat shift))).
+  assert (j < Zlength fs1 \/ j = Zlength fs1) as K by lia.
+  destruct K.
+  { replace (sublist j (Zlength fs1) fs1) with
+      (Znth j fs1 :: sublist (j + 1) (Zlength fs1) fs1) by list_solve.
+    unff listrepf.
+    subst.
+    Intros x y x1 y1.
+    entailer!. }
+  replace j with (Zlength fs1) by lia.
+  assert (i = Zlength fs2 \/ i < Zlength fs2) as K by lia.
+  destruct K.
+  { subst.
+    autorewrite with sublist norm.
+    unff listrepf.
+    Intros x y.
+    unnw; vauto. }
+  entailer!.
+  { rewrite <- filter_app.
+    replace (sublist 0 (Zlength fs1) fs1) with fs1 by list_solve.
+    rewrite fill_doc_app.
+    replace (sublist 0 (i + 1) fs2) with
+      (sublist 0 i fs2 ++ [Znth i fs2]) by list_solve.
+    vauto. }
+  autorewrite with sublist norm.
+  unff listrepf.
+  rewrite <- filter_app.
+  rewrite fill_doc_app.
+  replace (sublist 0 (i + 1) fs2) with
+    (sublist 0 i fs2 ++ [Znth i fs2]) by list_solve.
+  entailer!.
+  apply lsegf_null_listrepf. }
+assert (j = Zlength fs1 \/ j < Zlength fs1) as K by lia.
+destruct K.
+{ subst.
+  autorewrite with sublist norm.
+  unff listrepf.
+  Intros x y.
+  unnw; vauto. }
+assert (i = Zlength fs2 \/ i < Zlength fs2) as K by lia.
+destruct K.
+{ subst.
+  autorewrite with sublist norm.
+  unff listrepf.
+  Intros x y.
+  unnw; vauto. }
+replace (sublist i (Zlength fs2) fs2) with
+  (Znth i fs2 :: (sublist (i + 1) (Zlength fs2) fs2)) by list_solve.
+replace (sublist j (Zlength fs1) fs1) with
+  (Znth j fs1 :: (sublist (j + 1) (Zlength fs1) fs1)) by list_solve.
+unff listrepf.
+Intros ith_tail_fs1_ptr ith_format_fs1_ptr fs1_sigma fs1_sigma_pt.
+Intros ith_tail_fs2_ptr ith_format_fs2_ptr fs2_sigma fs2_sigma_pt.
+Intros nullval_ptr empty_ptr empty_sigma empty_sigma_pt.
+getnw; rewrite LIST_NULL_PTR.
+forward.
+{ entailer.
+  unfold concrete_mformat.
+  entailer!. }
+forward.
+{ entailer.
+  unfold concrete_mformat.
+  entailer!. }
+unfold concrete_mformat.
+Intros.
+forward_call(Znth j fs1, Znth i fs2, 
+    ith_format_fs1_ptr, ith_format_fs2_ptr, fs1_sigma, fs2_sigma, fs1_sigma_pt, fs2_sigma_pt, shift, gv).
+{ unfold concrete_mformat; entailer!. }
+{ getnw; inv FMT_MP; inv GOOD_FORMAT.
+  getnw; inv FMT_MP; inv GOOD_FORMAT.
+  getnw; inv FMT_MP; inv GOOD_FORMAT.  
+  split.
+  { destruct (Znth j fs1); ins.
+    destruct (Znth i fs2); ins.
+    apply mk_format_comb; ins.
+    all: unfold Int.max_unsigned in *.
+    all: ins.
+    all: lia. }
+  assert (Forall (fun x => 0 <= fst x + Zlength (snd x) <= w) fs2_sigma) as FORALL2.
+      { enough (list_max (map (fun x => Z.to_nat (fst x + Zlength (snd x))) fs2_sigma) <= Z.to_nat w)%nat.
+        { apply list_max_impl_forall; vauto. }
+        rewrite <- (total_width_eq (Znth i fs2)); vauto. }
+  assert (Forall (fun x => 0 <= fst x + Zlength (snd x) <= w) fs1_sigma) as FORALL1.
+      { enough (list_max (map (fun x => Z.to_nat (fst x + Zlength (snd x))) fs1_sigma) <= Z.to_nat w)%nat.
+        { apply list_max_impl_forall; vauto. }
+        rewrite <- (total_width_eq (Znth j fs1)); vauto. }
+  split.
+  { eapply beside_doc_llw_add.
+    4: eauto.
+    { lia. }
+    3: {
+      unfold total_width in *.
+      desf; ins; lia. }
+    all: inv format_mp_list_mp0.
+    all: vauto. }
+  eapply beside_doc_ab_pred.
+  4: eauto.
+  { lia. }
+  all: vauto. }
+Intros vret.
+destruct vret as (vret_sigma, result_sigma_pt).
+destruct vret_sigma as (result_format_ptr, result_sigma).
+forward.
+unfold concrete_mformat.
+Intros.
+forward_call(add_fill (Znth j fs1) (Znth i fs2) (Z.to_nat shift), result_format_ptr, result_sigma, result_sigma_pt, w, h).
+{ unfold concrete_mformat.
+  entailer!.
+  entailer!. }
+Intros width_check_result.
+forward_if(
+  EX res_part_new : list t, EX result_tail_ptr_new : val,
+  PROP(0 <= j <= Zlength fs1;
+        res_part_new = res_part ++ filter (fun G => (G.(height) <=? Z.to_nat h)%nat) (FormatTrivial.fillDoc (Z.to_nat w) (sublist 0 (j + 1) fs1) [Znth i fs2] (Z.to_nat shift)))
+  LOCAL(temp _fs2_tail head_ptr; temp _fs1_tail head_ptr2;
+        temp _has_item (Val.of_bool (0 <? Zlength res_part_new)); 
+        temp _result result_ptr; gvars gv; 
+        temp _shift (Vptrofs (Ptrofs.repr shift));
+        temp _width (Vint (Int.repr w)); temp _height (Vint (Int.repr h));
+        temp _fs1 p1; temp _fs2 p2; temp _result_tail result_tail_ptr_new)
+  SEP (mem_mgr gv; 
+      lsegf (sublist 0 j fs1) p1 head_ptr2 w h;
+      listrepf (sublist j (Zlength fs1) fs1) head_ptr2 w h;
+      lsegf (sublist 0 i fs2) p2 head_ptr w h; 
+      listrepf (sublist i (Zlength fs2) fs2) head_ptr w h; 
+      lsegf res_part_new result_ptr result_tail_ptr_new w h;
+      listrepf [empty] result_tail_ptr_new w h)).
+2: { forward.
+     { entailer!; unnw; desf. }
+     forward_call(result_sigma, result_sigma_pt, gv).
+     forward_call(t_format, result_format_ptr, gv).
+     { prove_ptr.
+       entailer!. }
+     Exists ((filter (fun G : t => (height G <=? Z.to_nat h)%nat)
+              (fillDoc (Z.to_nat w) fs1 (sublist 0 i fs2) (Z.to_nat shift)) ++
+              filter (fun G : t => (height G <=? Z.to_nat h)%nat)
+              (fillDoc (Z.to_nat w) (sublist 0 j fs1) [Znth i fs2] (Z.to_nat shift)))) result_tail_ptr_new.
+    entailer!.
+     2: {
+        unff listrepf.
+        Exists nullval empty_ptr empty_sigma empty_sigma_pt.
+        entailer!.  
+        unff concrete_mformat.
+        entailer!.
+        replace (sublist j (Zlength fs1) fs1) with 
+          (Znth j fs1 :: sublist (j + 1) (Zlength fs1) fs1) by list_solve.
+        unff listrepf.
+        Exists ith_tail_fs1_ptr ith_format_fs1_ptr fs1_sigma fs1_sigma_pt.
+        unfold concrete_mformat.
+        entailer!.
+        replace (sublist i (Zlength fs2) fs2) with 
+          (Znth i fs2 :: sublist (i + 1) (Zlength fs2) fs2) by list_solve.
+        unff listrepf.
+        Exists ith_tail_fs2_ptr ith_format_fs2_ptr fs2_sigma fs2_sigma_pt.
+        unfold concrete_mformat.
+        entailer!. }
+    replace (sublist 0 (j + 1) fs1) with (sublist 0 j fs1 ++ [Znth j fs1]) by list_solve.
+    rewrite <- fill_doc_app_l.
+    apply app_inv_head_iff.
+    rewrite filter_app.
+    enough(
+      filter (fun G : t => (height G <=? Z.to_nat h)%nat) (fillDoc (Z.to_nat w) [Znth j fs1] [Znth i fs2] (Z.to_nat shift)) = []
+    ) as K.
+    { rewrite K; list_solve. }
+    unfold FormatTrivial.fillDoc.
+    unfold FormatTrivial.cross_general.
+    rewrite map_cons.
+    rewrite concat_cons.
+    rewrite map_nil.
+    rewrite concat_nil.
+    autorewrite with sublist norm.
+    unfold filter.
+    desf; vauto.
+    lia. }
+2: {
+  Intros res_part_new0 result_tail_ptr_new0.
+  replace (sublist j (Zlength fs1) fs1) with 
+    (Znth j fs1 :: sublist (j + 1) (Zlength fs1) fs1) by list_solve.  
+  unff listrepf.
+  Intros ith_tail_fs1_ptr_new ith_format_fs1_ptr_new fs1_sigma_new fs1_sigma_pt_new.
+  Intros empty_ptr_new empty_format_ptr_new empty_sigma_new empty_sigma_pt_new.
+  forward.
+  { entailer!; unnw; desf. }
+  rewrite eqn_loop.
+  Exists (j + 1) ith_tail_fs1_ptr_new result_tail_ptr_new0 res_part_new0.
+  entailer!.
+  unff listrepf.
+  Exists empty_ptr_new empty_format_ptr_new empty_sigma_new empty_sigma_pt_new.
+  unfold concrete_mformat.
+  entailer!.
+  assert (
+    lsegf (sublist 0 j fs1) p1 head_ptr2 w h *
+    lsegf [Znth j fs1] head_ptr2 ith_tail_fs1_ptr_new w h |--
+    lsegf (sublist 0 (j + 1) fs1) p1 ith_tail_fs1_ptr_new w h
+  ) as K.
+  { replace (sublist 0 (j + 1) fs1) with
+      (sublist 0 j fs1 ++ [Znth j fs1]) by list_solve.
+    apply lsegf_lsegf. }
+  eapply derives_trans.
+  2: eauto.
+  entailer!.
+  unff lsegf.
+  Exists ith_tail_fs1_ptr_new ith_format_fs1_ptr_new fs1_sigma_new fs1_sigma_pt_new.
+  entailer!.
+  unfold concrete_mformat.
+  entailer!. } 
+do 2 forward.
+{ entailer!; unnw; desf. }
+forward_call(empty_sigma, empty_sigma_pt, gv).
+forward.
+forward_call(t_format, empty_ptr, gv).
+{ prove_ptr; entailer!. }
+forward.
+forward_call(t_flist, gv).
+Intros new_result_tail_ptr.
+do 2 forward.
+dest_ptr new_result_tail_ptr.
+forward_call(gv).
+Intros new_empty_ptr.
+do 6 forward.
+Exists (filter (fun G : t => (height G <=? Z.to_nat h)%nat)
+        (fillDoc (Z.to_nat w) fs1 (sublist 0 i fs2) (Z.to_nat shift)) ++
+        filter (fun G : t => (height G <=? Z.to_nat h)%nat)
+        (fillDoc (Z.to_nat w) (sublist 0 (j + 1) fs1) [Znth i fs2] (Z.to_nat shift))) new_result_tail_ptr.
+entailer!.
+2: { 
+  unfold mformat.
+  Intros sigma0 sigma_pt0.
+  unff listrepf.
+  Exists nullval new_empty_ptr sigma0 sigma_pt0.
+  unfold concrete_mformat.
+  entailer!.
+  remember ((filter (fun G : t => (height G <=? Z.to_nat h)%nat) (fillDoc (Z.to_nat w) fs1 (sublist 0 i fs2) (Z.to_nat shift)))) as part1.
+  remember (filter (fun G : t => (height G <=? Z.to_nat h)%nat) (fillDoc (Z.to_nat w) (sublist 0 j fs1) [Znth i fs2] (Z.to_nat shift))) as part2.
+  remember (filter (fun G : t => (height G <=? Z.to_nat h)%nat) (fillDoc (Z.to_nat w) (sublist 0 (j + 1) fs1) [Znth i fs2] (Z.to_nat shift))) as part3.
+  remember (filter (fun G : t => (height G <=? Z.to_nat h)%nat) (fillDoc (Z.to_nat w) [Znth j fs1] [Znth i fs2] (Z.to_nat shift))) as part4.
+  assert (part1 ++ part3 = (part1 ++ part2) ++ part4) as K.
+  { rewrite <- app_assoc.
+    apply app_inv_head_iff.
+    vauto.
+    replace (sublist 0 (j + 1) fs1) with (sublist 0 j fs1 ++ [Znth j fs1]) by list_solve.
+    rewrite <- fill_doc_app_l.
+    rewrite filter_app; vauto. }
+  rewrite K.
+  assert(
+    listrepf (sublist j (Zlength fs1) fs1) head_ptr2 w h
+    * listrepf (sublist i (Zlength fs2) fs2) head_ptr w h
+    * lsegf (part1 ++ part2) result_ptr result_tail_ptr_new w h
+    * lsegf part4 result_tail_ptr_new new_result_tail_ptr w h |--
+    listrepf (sublist j (Zlength fs1) fs1) head_ptr2 w h
+      * listrepf (sublist i (Zlength fs2) fs2) head_ptr w h
+      * lsegf ((part1 ++ part2) ++ part4) result_ptr new_result_tail_ptr w h
+  ) as FF.
+  { entailer!.
+    apply lsegf_lsegf. }
+  eapply derives_trans.
+  2: eauto.
+  entailer!.
+  unfold FormatTrivial.fillDoc.
+  unfold FormatTrivial.cross_general.
+  rewrite map_cons.
+  rewrite map_nil.
+  rewrite map_cons.
+  rewrite map_nil.
+  rewrite concat_cons.
+  rewrite concat_nil.
+  autorewrite with sublist.
+  unfold filter.
+  desf;
+  assert (
+    (total_width (add_fill (Znth j fs1) (Znth i fs2) (Z.to_nat shift)) <= Z.to_nat w)%nat /\
+      (height (add_fill (Znth j fs1) (Znth i fs2) (Z.to_nat shift)) <= Z.to_nat h)%nat
+  ) as GG by auto; desf.
+  unff lsegf.
+  Exists new_result_tail_ptr result_format_ptr result_sigma result_sigma_pt.
+  entailer!.
+  { unfold good_format; split; vauto. }
+  unfold concrete_mformat; entailer!.
+  assert (
+    listrepf (sublist j (Zlength fs1) fs1) head_ptr2 w h
+    * lsegf [Znth i fs2] head_ptr ith_tail_fs2_ptr w h
+    * listrepf (sublist (i + 1) (Zlength fs2) fs2) ith_tail_fs2_ptr w h |--
+    listrepf (sublist j (Zlength fs1) fs1) head_ptr2 w h
+    * listrepf (sublist i (Zlength fs2) fs2) head_ptr w h
+  ) as KK.
+  { entailer!.
+    replace (sublist i (Zlength fs2) fs2) 
+      with ([Znth i fs2] ++ sublist (i + 1) (Zlength fs2) fs2) by list_solve.
+    apply lsegf_listf. }
+  eapply derives_trans.
+  2: eauto.
+  entailer!.
+  unff lsegf.
+  Exists ith_tail_fs2_ptr ith_format_fs2_ptr fs2_sigma fs2_sigma_pt.
+  unfold concrete_mformat.
+  entailer!.
+  assert(
+    lsegf [Znth j fs1] head_ptr2 ith_tail_fs1_ptr w h
+    * listrepf (sublist (j + 1) (Zlength fs1) fs1) ith_tail_fs1_ptr w h |--
+    listrepf (sublist j (Zlength fs1) fs1) head_ptr2 w h
+  ) as KKK.
+  { replace (sublist j (Zlength fs1) fs1) with
+      ([Znth j fs1] ++ sublist (j + 1) (Zlength fs1) fs1) by list_solve.
+    apply lsegf_listf. }
+  eapply derives_trans.
+  2: eauto.
+  entailer!.
+  unff lsegf.
+  Exists ith_tail_fs1_ptr ith_format_fs1_ptr fs1_sigma fs1_sigma_pt.
+  unfold concrete_mformat.
+  entailer!. }
+autorewrite with sublist norm.
+desf.
+remember (filter (fun G : t => (height G <=? Z.to_nat h)%nat) (fillDoc (Z.to_nat w) (sublist 0 j fs1) [Znth i fs2] (Z.to_nat shift))) as part2.
+remember ((filter (fun G : t => (height G <=? Z.to_nat h)%nat) (fillDoc (Z.to_nat w) fs1 (sublist 0 i fs2) (Z.to_nat shift)))) as part1.
+remember (filter (fun G : t => (height G <=? Z.to_nat h)%nat) (fillDoc (Z.to_nat w) (sublist 0 (j + 1) fs1) [Znth i fs2] (Z.to_nat shift))) as part3.
+remember (filter (fun G : t => (height G <=? Z.to_nat h)%nat) (fillDoc (Z.to_nat w) [Znth j fs1] [Znth i fs2] (Z.to_nat shift))) as part4.
+assert (part3 = part2 ++ part4) as K.
+{ vauto.
+  replace (sublist 0 (j + 1) fs1) with (sublist 0 j fs1 ++ [Znth j fs1]) by list_solve.
+  rewrite <- fill_doc_app_l.
+  rewrite filter_app; vauto. }
+rewrite K.
+rewrite Zlength_app.
+enough (Zlength part4 = 1) as KK. 
+{ rewrite KK.
+  assert(Zlength part1 + Zlength part2 + 1 > 0) as FF.
+  { list_solve. }
+  assert (0 <? Zlength part1 + (Zlength part2 + 1) = true) as GG.
+  { lia. }
+  rewrite GG.
+  list_solve. }
+vauto.
+unfold fillDoc.
+unfold cross_general.
+rewrite map_cons.
+rewrite map_nil.
+rewrite map_cons.
+rewrite map_nil.
+rewrite concat_cons.
+rewrite concat_nil.
+autorewrite with sublist.
+unfold filter.
+desf;
+assert (
+  (total_width (add_fill (Znth j fs1) (Znth i fs2) (Z.to_nat shift)) <= Z.to_nat w)%nat /\
+    (height (add_fill (Znth j fs1) (Znth i fs2) (Z.to_nat shift)) <= Z.to_nat h)%nat
+) as GG by auto; desf.
+Qed.
+
+
+Lemma body_above_doc: semax_body Vprog Gprog f_above_doc above_doc_spec.
+Proof.
+  start_function.
+  forward_if(p1 <> nullval).
+  { forward_if(
+    PROP ( )
+    LOCAL (gvars gv; temp _width (Vint (Int.repr w)); temp _height (Vint (Int.repr h)); temp _fs1 p1; temp _fs2 p2)
+    SEP (listrepf fs1 p1 w h; mem_mgr gv)).
+    { forward_call(fs2, p2, w, h, gv); entailer!. }
+    { forward; entailer!. 
+      unnw; desf.
+      assert (fs2 = []) by auto; subst.
+      unff listrepf; entailer!. }
+    forward.
+    unnw; desf.
+    assert (fs1 = []) by auto; subst.
+    Exists nullval ([] : list t); entailer!.
+    unfold FormatTrivial.aboveDoc.
+    unfold FormatTrivial.cross_general; ins.
+    rewrite concat_map_nil; list_solve. }
+  { forward; entailer!. }
+
+  forward_if(p2 <> nullval).
+  { forward_call(fs1, p1, w, h, gv).
+    forward.
+    unnw; desf.
+    assert (fs2 = []) by auto; subst.
+    Exists nullval ([] : list t); entailer!. }
+  { forward; entailer!. }
+  forward_call(t_flist, gv).
+  Intros result_ptr.
+  dest_ptr result_ptr.
+  forward_call(gv).
+  Intros cur_empty_ptr.
+  do 3 forward.
+  desf.
+  do 2 forward.
+  
+
+  remember (
+      EX i : Z, EX head_ptr : val, EX result_tail_ptr : val, EX res_part : list t,
+      PROP(0 <= i <= Zlength fs2;
+            res_part = filter (fun G => (G.(height) <=? Z.to_nat h)%nat) (FormatTrivial.aboveDoc (Z.to_nat w) fs1 (sublist 0 i fs2)))
+      LOCAL(temp _fs2_tail head_ptr;
+            temp _has_item (Val.of_bool (0 <? Zlength res_part)); temp _result result_ptr; gvars gv; 
+            temp _width (Vint (Int.repr w)); temp _height (Vint (Int.repr h));
+            temp _fs1 p1; temp _fs2 p2; temp _result_tail result_tail_ptr)
+      SEP (mem_mgr gv; listrepf fs1 p1 w h; lsegf (sublist 0 i fs2) p2 head_ptr w h; 
+          listrepf (sublist i (Zlength fs2) fs2) head_ptr w h; lsegf res_part result_ptr result_tail_ptr w h;
+          listrepf [empty] result_tail_ptr w h)) as loop_invariant eqn:eqn_loop.
+  remember (
+      EX result_tail_ptr : val, EX res_part : list t,
+      PROP(res_part = filter (fun G => (G.(height) <=? Z.to_nat h)%nat) (FormatTrivial.aboveDoc (Z.to_nat w) fs1 fs2))
+      LOCAL(temp _has_item (Val.of_bool (0 <? Zlength res_part)); temp _result result_ptr; gvars gv;
+            temp _result_tail result_tail_ptr;
+            temp _width (Vint (Int.repr w)); temp _height (Vint (Int.repr h));
+            temp _fs1 p1; temp _fs2 p2)
+      SEP (mem_mgr gv; listrepf fs1 p1 w h; listrepf fs2 p2 w h; lsegf res_part result_ptr result_tail_ptr w h;
+          listrepf [empty] result_tail_ptr w h)) as break_invariant eqn:eqn_break.
+  forward_loop(loop_invariant) break: (break_invariant).
+  { subst.
+    Exists 0 p2 result_ptr ([] : list t).
+    entailer!.
+    replace (sublist 0 0 fs2) with ([] : list t) by list_solve.
+    assert (sublist 0 (Zlength fs2) fs2 = fs2) as K.
+    { rewrite sublist_skip; vauto. }
+    rewrite K.
+    unff lsegf; entailer!; ins.
+    unfold mformat.
+    Intros sigma_list sigma_pt.
+    unff listrepf.
+    Exists nullval cur_empty_ptr sigma_list sigma_pt.
+    unfold concrete_mformat.
+    entailer!.
+    getnw.
+    inv FMT_MP.
+    unfold empty in *; ins.
+    unnw; unfold good_format; ins.
+    assert (sigma_list = []) by list_solve; subst.
+    list_solve. }
+  2: { subst.
+      Intros result_tail_ptr res_part.
+      forward_call(fs1, p1, w, h, gv).
+      forward_call(fs2, p2, w, h, gv).
+      forward_if (
+        Zlength res_part <> 0
+      ).
+      { destruct (0 <? Zlength res_part) eqn:E; vauto.
+        forward_call([empty], result_ptr, w, h, gv).
+        { desf; entailer!.
+          replace ((filter (fun G : t => (height G <=? Z.to_nat h)%nat)
+          (FormatTrivial.aboveDoc (Z.to_nat w) fs1 fs2))) with ([] : list t) by list_solve.
+          unff lsegf; unff listrepf.
+          entailer!; subst; unnw; entailer!.
+          Exists nullval y format_sigma sigma_pt; entailer!. }
+        forward.
+        Exists nullval ([] : list t); entailer!.
+        2: { unff listrepf; entailer!. }
+        list_solve. }
+      { forward; entailer!; ins.
+        assert (Zlength (filter (fun G : t => (height G <=? Z.to_nat h)%nat)
+           (FormatTrivial.aboveDoc (Z.to_nat w) fs1 fs2)) = 0) as K by vauto.
+        rewrite K in *; vauto. }
+      forward.
+      forward_loop(
+        EX i : Z, EX new_result_tail : val,
+        PROP(0 <= i < Zlength res_part)
+        LOCAL(temp _new_result_tail new_result_tail; temp _fs1 p1; temp _fs2 p2; 
+              temp _result_tail result_tail_ptr; gvars gv; temp _result result_ptr)
+        SEP(mem_mgr gv; lsegf (sublist 0 i res_part) result_ptr new_result_tail w h; 
+            listrepf (sublist i (Zlength res_part) res_part ++ [empty]) new_result_tail w h)
+      ) break: (
+        EX new_result_tail : val,
+        PROP()
+        LOCAL(temp _new_result_tail new_result_tail; temp _fs1 p1; temp _fs2 p2; 
+              temp _result_tail result_tail_ptr; gvars gv; temp _result result_ptr)
+        SEP(mem_mgr gv; lsegf (sublist 0 (Zlength res_part - 1) res_part) result_ptr new_result_tail w h; 
+            listrepf (sublist (Zlength res_part - 1) (Zlength res_part) res_part ++ [empty]) new_result_tail w h)).
+      { Exists 0 result_ptr.
+        entailer!.
+        autorewrite with sublist.
+        unff lsegf; entailer!.
+        apply lsegf_listf. }
+      { Intros i new_result_tail_ptr.
+        replace (sublist i (Zlength res_part) res_part) with (Znth i res_part :: sublist (i + 1) (Zlength res_part) res_part)
+          by list_solve.
+        autorewrite with sublist norm.
+        replace ((Znth i res_part
+            :: sublist (i + 1) (Zlength res_part) res_part) ++ [empty]) with
+            (Znth i res_part :: (sublist (i + 1) (Zlength res_part) res_part ++ [empty])) by list_solve.
+        unff listrepf.
+        Intros ith_tail_ptr ith_format_ptr format_sigma sigma_pt.
+        forward.
+        { entailer!; getnw; desf. }
+        assert (i + 1 = Zlength res_part \/ i + 1 < Zlength res_part) as K by lia.
+        destruct K.
+        { replace (sublist (i + 1) (Zlength res_part) res_part) with ([] : list t) by list_solve.
+          autorewrite with sublist.
+          unff listrepf.
+          Intros nullval_tail_ptr empty_ptr format_sigma_empty sigma_pt_empty.
+          forward.
+          { unnw; subst; entailer!. }
+          getnw; rewrite LIST_NULL_PTR.
+          forward_if.
+          { vauto. }
+          forward.  
+          entailer!.
+          Exists new_result_tail_ptr.
+          remember (filter (fun G : t => (height G <=? Z.to_nat h)%nat) (FormatTrivial.aboveDoc (Z.to_nat w) fs1 fs2))
+            as res_part.
+          replace i with (Zlength res_part - 1) by lia.
+          replace (sublist (Zlength res_part - 1) (Zlength res_part) res_part ++ [empty])
+            with [Znth (Zlength res_part - 1) res_part; empty] by list_solve.
+          unff listrepf.
+          Exists ith_tail_ptr ith_format_ptr format_sigma sigma_pt.
+          Exists nullval empty_ptr format_sigma_empty sigma_pt_empty.
+          entailer!.
+          unnw.
+          list_solve. }
+        replace (sublist (i + 1) (Zlength res_part) res_part)
+          with (Znth (i + 1) res_part :: sublist (i + 2) (Zlength res_part) res_part) by list_solve.
+        replace ((Znth (i + 1) res_part :: sublist (i + 2) (Zlength res_part) res_part) ++ [empty]) with
+            (Znth (i + 1) res_part :: ((sublist (i + 2) (Zlength res_part) res_part ++ [empty]))) by list_solve.
+        unff listrepf.
+        Intros ithplus_tail_ptr ithplus_format_ptr ith_plus_sigma ith_plus_sigma_pt.
+        forward.
+        { entailer!; unnw; desf.  }
+        forward_if.
+        { forward; entailer!.
+          remember (filter (fun G : t => (height G <=? Z.to_nat h)%nat) (FormatTrivial.aboveDoc (Z.to_nat w) fs1 fs2)).
+          Exists (i + 1) ith_tail_ptr.
+          replace (sublist (i + 1) (Zlength l) l) with
+              (Znth (i + 1) l :: sublist (i + 2) (Zlength l) l) by list_solve.
+          replace ((Znth (i + 1) l :: sublist (i + 2) (Zlength l) l) ++ [empty]) with 
+              (Znth (i + 1) l :: (sublist (i + 2) (Zlength l) l ++ [empty])) by list_solve.
+          unff listrepf.
+          Exists ithplus_tail_ptr ithplus_format_ptr ith_plus_sigma ith_plus_sigma_pt.
+          entailer!.
+          remember (filter (fun G : t => (height G <=? Z.to_nat h)%nat) (FormatTrivial.aboveDoc (Z.to_nat w) fs1 fs2)).
+          assert (
+            lsegf (sublist 0 i l) result_ptr new_result_tail_ptr w h *
+            lsegf [Znth i l] new_result_tail_ptr ith_tail_ptr w h |--
+            lsegf (sublist 0 (i + 1) l) result_ptr ith_tail_ptr w h) as K.
+          { replace (sublist 0 (i + 1) l) with (sublist 0 i l ++ [Znth i l]) by list_solve.
+            eapply lsegf_lsegf. }
+          eapply derives_trans.
+          2: eauto.
+          entailer!.
+          unff lsegf; Exists ith_tail_ptr ith_format_ptr format_sigma sigma_pt.
+          entailer!. }
+        forward.
+        replace ithplus_tail_ptr with nullval by vauto.
+        destruct (sublist (i + 2) (Zlength res_part) res_part).
+        { autorewrite with sublist norm.
+          unff listrepf.
+          Intros x y format_sigma0 sigma_pt0.
+          entailer!. }
+        replace (((t :: l) ++ [empty])) with (t :: (l ++ [empty])) by list_solve.
+        unff listrepf.
+        Intros x y format_sigma0 sigma_pt0.
+        entailer!. }
+    Intros new_result_tail.
+    replace (sublist (Zlength res_part - 1) (Zlength res_part) res_part ++ [empty]) with 
+        [Znth (Zlength res_part - 1) res_part; empty] by list_solve.
+    unff listrepf.
+    Intros empty_list_ptr last_format_ptr empty_sigma empty_sigma_ptr.
+    Intros nullval_ptr empty_format_ptr format_sigma0 sigma_pt0.
+    forward.
+    forward_call([empty], empty_list_ptr, w, h, gv).
+    { getnw; subst.
+      unff listrepf.
+      Exists nullval empty_format_ptr format_sigma0 sigma_pt0.
+      entailer!. }
+    do 2 forward.
+    Exists result_ptr (filter (fun G : t => (height G <=? Z.to_nat h)%nat) (FormatTrivial.aboveDoc (Z.to_nat w) fs1 fs2)).
+    entailer!.
+    remember (filter (fun G : t => (height G <=? Z.to_nat h)%nat) (FormatTrivial.aboveDoc (Z.to_nat w) fs1 fs2)).
+    assert (
+      lsegf (sublist 0 (Zlength l - 1) l) result_ptr new_result_tail w h *
+      listrepf [Znth (Zlength l - 1) l] new_result_tail w h |--
+      listrepf l result_ptr w h
+    ) as K.
+    { assert(l = (sublist 0 (Zlength l - 1) l ++ [Znth (Zlength l - 1) l])) as KK by list_solve.
+      rewrite KK at 5.
+      apply lsegf_listf. }
+    eapply derives_trans.
+    2: eauto.
+    unff listrepf.
+    Exists nullval last_format_ptr empty_sigma empty_sigma_ptr.
+    entailer!. }
+subst.
+Intros i head_ptr result_tail_ptr res_part.
+forward_if.
+2: {
+  forward.
+  Exists result_tail_ptr res_part.
+  assert(i < Zlength fs2 \/ i = Zlength fs2) as K by lia.
+  destruct K.
+  { replace (sublist i (Zlength fs2) fs2) with 
+      (Znth i fs2 :: sublist (i + 1) (Zlength fs2) fs2) by list_solve.
+    unff listrepf.
+    Intros x1 y1 x2 y2.
+    subst.
+    entailer!. }
+  entailer!.
+  { autorewrite with sublist norm; vauto. }
+  autorewrite with sublist norm.
+  unff listrepf.
+  entailer!.
+  apply lsegf_null_listrepf. }
+forward.
+remember (
+    EX j : Z, EX head_ptr2 : val, EX result_tail_ptr_new : val, EX res_part_new : list t,
+    PROP(0 <= j <= Zlength fs1;
+          res_part_new = res_part ++ filter (fun G => (G.(height) <=? Z.to_nat h)%nat) (FormatTrivial.aboveDoc (Z.to_nat w) (sublist 0 j fs1) [Znth i fs2]))
+    LOCAL(temp _fs2_tail head_ptr; temp _fs1_tail head_ptr2;
+          temp _has_item (Val.of_bool (0 <? Zlength res_part_new)); 
+          temp _result result_ptr; gvars gv; 
+          temp _width (Vint (Int.repr w)); temp _height (Vint (Int.repr h));
+          temp _fs1 p1; temp _fs2 p2; temp _result_tail result_tail_ptr_new)
+    SEP (mem_mgr gv; 
+        lsegf (sublist 0 j fs1) p1 head_ptr2 w h;
+        listrepf (sublist j (Zlength fs1) fs1) head_ptr2 w h;
+        lsegf (sublist 0 i fs2) p2 head_ptr w h; 
+        listrepf (sublist i (Zlength fs2) fs2) head_ptr w h; 
+        lsegf res_part_new result_ptr result_tail_ptr_new w h;
+        listrepf [empty] result_tail_ptr_new w h)) as loop_invariant eqn:eqn_loop.
+remember (
+    EX result_tail_ptr_new : val, EX res_part_new : list t,
+    PROP(res_part_new = filter (fun G => (G.(height) <=? Z.to_nat h)%nat) (FormatTrivial.aboveDoc (Z.to_nat w) fs1 (sublist 0 (i + 1) fs2)))
+    LOCAL(temp _has_item (Val.of_bool (0 <? Zlength res_part_new)); 
+          temp _result result_ptr; 
+          gvars gv;
+          temp _result_tail result_tail_ptr_new;
+          temp _width (Vint (Int.repr w)); temp _height (Vint (Int.repr h));
+          temp _fs1 p1; temp _fs2 p2;
+          temp _fs2_tail head_ptr)
+    SEP (mem_mgr gv; 
+        listrepf fs1 p1 w h; 
+        lsegf (sublist 0 i fs2) p2 head_ptr w h; 
+        listrepf (sublist i (Zlength fs2) fs2) head_ptr w h; 
+        lsegf res_part_new result_ptr result_tail_ptr_new w h;
+        listrepf [empty] result_tail_ptr_new w h)) as break_invariant eqn:eqn_break.
+forward_loop(loop_invariant) break: (break_invariant).
+{ rewrite eqn_loop.
+  Exists 0 p1 result_tail_ptr res_part.
+  entailer!.
+  { autorewrite with sublist norm; vauto. }
+  autorewrite with sublist norm.
+  unff lsegf; entailer!. }
+2: {
+  rewrite eqn_break.
+  Intros result_tail_ptr_new res_part_new.
+  assert(i = Zlength fs2 \/ i < Zlength fs2) as K by lia.
+  destruct K.
+  { subst.
+    autorewrite with sublist norm.
+    unff listrepf.
+    Intros; unnw; vauto. }
+  replace (sublist i (Zlength fs2) fs2) 
+    with (Znth i fs2 :: (sublist (i + 1) (Zlength fs2) fs2)) by list_solve.
+  unff listrepf.
+  Intros ith_tail_ptr ith_format_ptr ith_sigma ith_sigma_pt.
+  Intros nullval_ptr empty_ptr empty_sigma empty_sigma_pt.
+  getnw; rewrite LIST_NULL_PTR.
+  forward.
+  { entailer!; unnw; desf. }
+  Exists (i + 1) ith_tail_ptr result_tail_ptr_new res_part_new.
+  entailer!.
+  unff listrepf.
+  Exists nullval empty_ptr empty_sigma empty_sigma_pt.
+  entailer!.
+  assert (
+    lsegf (sublist 0 i fs2) p2 head_ptr w h *
+    lsegf [Znth i fs2] head_ptr ith_tail_ptr w h |--
+    lsegf (sublist 0 (i + 1) fs2) p2 ith_tail_ptr w h
+  ) as K.
+  { replace (sublist 0 (i + 1) fs2) with
+      (sublist 0 i fs2 ++ [Znth i fs2]) by list_solve.
+    apply lsegf_lsegf. }
+  eapply derives_trans.
+  2: eauto.
+  entailer!.
+  unff lsegf; entailer!.
+  Exists ith_tail_ptr ith_format_ptr ith_sigma ith_sigma_pt.
+  entailer!. }
+rewrite eqn_loop.
+Intros j head_ptr2 result_tail_ptr_new res_part_new.
+forward_if.
+2: { 
+  forward.
+  rewrite eqn_break.
+  Exists result_tail_ptr_new 
+    (filter (fun G : t => (height G <=? Z.to_nat h)%nat) (FormatTrivial.aboveDoc (Z.to_nat w) fs1 (sublist 0 (i + 1) fs2))).
+  assert (j < Zlength fs1 \/ j = Zlength fs1) as K by lia.
+  destruct K.
+  { replace (sublist j (Zlength fs1) fs1) with
+      (Znth j fs1 :: sublist (j + 1) (Zlength fs1) fs1) by list_solve.
+    unff listrepf.
+    subst.
+    Intros x y x1 y1.
+    entailer!. }
+  replace j with (Zlength fs1) by lia.
+  assert (i = Zlength fs2 \/ i < Zlength fs2) as K by lia.
+  destruct K.
+  { subst.
+    autorewrite with sublist norm.
+    unff listrepf.
+    Intros x y.
+    unnw; vauto. }
+  entailer!.
+  { rewrite <- filter_app.
+    replace (sublist 0 (Zlength fs1) fs1) with fs1 by list_solve.
+    rewrite above_doc_app.
+    replace (sublist 0 (i + 1) fs2) with
+      (sublist 0 i fs2 ++ [Znth i fs2]) by list_solve.
+    vauto. }
+  autorewrite with sublist norm.
+  unff listrepf.
+  rewrite <- filter_app.
+  rewrite above_doc_app.
+  replace (sublist 0 (i + 1) fs2) with
+    (sublist 0 i fs2 ++ [Znth i fs2]) by list_solve.
+  entailer!.
+  apply lsegf_null_listrepf. }
+assert (j = Zlength fs1 \/ j < Zlength fs1) as K by lia.
+destruct K.
+{ subst.
+  autorewrite with sublist norm.
+  unff listrepf.
+  Intros x y.
+  unnw; vauto. }
+assert (i = Zlength fs2 \/ i < Zlength fs2) as K by lia.
+destruct K.
+{ subst.
+  autorewrite with sublist norm.
+  unff listrepf.
+  Intros x y.
+  unnw; vauto. }
+replace (sublist i (Zlength fs2) fs2) with
+  (Znth i fs2 :: (sublist (i + 1) (Zlength fs2) fs2)) by list_solve.
+replace (sublist j (Zlength fs1) fs1) with
+  (Znth j fs1 :: (sublist (j + 1) (Zlength fs1) fs1)) by list_solve.
+unff listrepf.
+Intros ith_tail_fs1_ptr ith_format_fs1_ptr fs1_sigma fs1_sigma_pt.
+Intros ith_tail_fs2_ptr ith_format_fs2_ptr fs2_sigma fs2_sigma_pt.
+Intros nullval_ptr empty_ptr empty_sigma empty_sigma_pt.
+getnw; rewrite LIST_NULL_PTR.
+forward.
+{ entailer.
+  unfold concrete_mformat.
+  entailer!. }
+forward.
+{ entailer.
+  unfold concrete_mformat.
+  entailer!. }
+unfold concrete_mformat.
+Intros.
+forward_call(Znth j fs1, Znth i fs2, 
+    ith_format_fs1_ptr, ith_format_fs2_ptr, fs1_sigma, fs2_sigma, fs1_sigma_pt, fs2_sigma_pt, gv).
+{ unfold concrete_mformat; entailer!. }
+{ getnw; inv FMT_MP; inv GOOD_FORMAT.
+  getnw; inv FMT_MP; inv GOOD_FORMAT.
+  getnw; inv FMT_MP; inv GOOD_FORMAT.  
+  destruct (Znth j fs1); ins.
+  destruct (Znth i fs2); ins.
+  apply mk_format_comb; ins.
+  all: unfold Int.max_unsigned in *.
+  all: ins.
+  all: lia. }
+Intros vret.
+destruct vret as (vret_sigma, result_sigma_pt).
+destruct vret_sigma as (result_format_ptr, result_sigma).
+forward.
+unfold concrete_mformat.
+Intros.
+forward_call(add_above (Znth j fs1) (Znth i fs2), result_format_ptr, result_sigma, result_sigma_pt, w, h).
+{ unfold concrete_mformat.
+  entailer!.
+  entailer!. }
+Intros width_check_result.
+forward_if(
+  EX res_part_new : list t, EX result_tail_ptr_new : val,
+  PROP(0 <= j <= Zlength fs1;
+        res_part_new = res_part ++ filter (fun G => (G.(height) <=? Z.to_nat h)%nat) (FormatTrivial.aboveDoc (Z.to_nat w) (sublist 0 (j + 1) fs1) [Znth i fs2]))
+  LOCAL(temp _fs2_tail head_ptr; temp _fs1_tail head_ptr2;
+        temp _has_item (Val.of_bool (0 <? Zlength res_part_new)); 
+        temp _result result_ptr; gvars gv; 
+        temp _width (Vint (Int.repr w)); temp _height (Vint (Int.repr h));
+        temp _fs1 p1; temp _fs2 p2; temp _result_tail result_tail_ptr_new)
+  SEP (mem_mgr gv; 
+      lsegf (sublist 0 j fs1) p1 head_ptr2 w h;
+      listrepf (sublist j (Zlength fs1) fs1) head_ptr2 w h;
+      lsegf (sublist 0 i fs2) p2 head_ptr w h; 
+      listrepf (sublist i (Zlength fs2) fs2) head_ptr w h; 
+      lsegf res_part_new result_ptr result_tail_ptr_new w h;
+      listrepf [empty] result_tail_ptr_new w h)).
+2: { forward.
+     { entailer!; unnw; desf. }
+     forward_call(result_sigma, result_sigma_pt, gv).
+     forward_call(t_format, result_format_ptr, gv).
+     { prove_ptr.
+       entailer!. }
+     Exists ((filter (fun G : t => (height G <=? Z.to_nat h)%nat)
+              (aboveDoc (Z.to_nat w) fs1 (sublist 0 i fs2)) ++
+              filter (fun G : t => (height G <=? Z.to_nat h)%nat)
+              (aboveDoc (Z.to_nat w) (sublist 0 j fs1) [Znth i fs2]))) result_tail_ptr_new.
+    entailer!.
+     2: {
+        unff listrepf.
+        Exists nullval empty_ptr empty_sigma empty_sigma_pt.
+        entailer!.  
+        unff concrete_mformat.
+        entailer!.
+        replace (sublist j (Zlength fs1) fs1) with 
+          (Znth j fs1 :: sublist (j + 1) (Zlength fs1) fs1) by list_solve.
+        unff listrepf.
+        Exists ith_tail_fs1_ptr ith_format_fs1_ptr fs1_sigma fs1_sigma_pt.
+        unfold concrete_mformat.
+        entailer!.
+        replace (sublist i (Zlength fs2) fs2) with 
+          (Znth i fs2 :: sublist (i + 1) (Zlength fs2) fs2) by list_solve.
+        unff listrepf.
+        Exists ith_tail_fs2_ptr ith_format_fs2_ptr fs2_sigma fs2_sigma_pt.
+        unfold concrete_mformat.
+        entailer!. }
+    replace (sublist 0 (j + 1) fs1) with (sublist 0 j fs1 ++ [Znth j fs1]) by list_solve.
+    rewrite <- above_doc_app_l.
+    apply app_inv_head_iff.
+    rewrite filter_app.
+    enough(
+      filter (fun G : t => (height G <=? Z.to_nat h)%nat) (aboveDoc (Z.to_nat w) [Znth j fs1] [Znth i fs2]) = []
+    ) as K.
+    { rewrite K; list_solve. }
+    unfold FormatTrivial.aboveDoc.
+    unfold FormatTrivial.cross_general.
+    rewrite map_cons.
+    rewrite concat_cons.
+    rewrite map_nil.
+    rewrite concat_nil.
+    autorewrite with sublist norm.
+    unfold filter.
+    desf; vauto.
+    lia. }
+2: {
+  Intros res_part_new0 result_tail_ptr_new0.
+  replace (sublist j (Zlength fs1) fs1) with 
+    (Znth j fs1 :: sublist (j + 1) (Zlength fs1) fs1) by list_solve.  
+  unff listrepf.
+  Intros ith_tail_fs1_ptr_new ith_format_fs1_ptr_new fs1_sigma_new fs1_sigma_pt_new.
+  Intros empty_ptr_new empty_format_ptr_new empty_sigma_new empty_sigma_pt_new.
+  forward.
+  { entailer!; unnw; desf. }
+  rewrite eqn_loop.
+  Exists (j + 1) ith_tail_fs1_ptr_new result_tail_ptr_new0 res_part_new0.
+  entailer!.
+  unff listrepf.
+  Exists empty_ptr_new empty_format_ptr_new empty_sigma_new empty_sigma_pt_new.
+  unfold concrete_mformat.
+  entailer!.
+  assert (
+    lsegf (sublist 0 j fs1) p1 head_ptr2 w h *
+    lsegf [Znth j fs1] head_ptr2 ith_tail_fs1_ptr_new w h |--
+    lsegf (sublist 0 (j + 1) fs1) p1 ith_tail_fs1_ptr_new w h
+  ) as K.
+  { replace (sublist 0 (j + 1) fs1) with
+      (sublist 0 j fs1 ++ [Znth j fs1]) by list_solve.
+    apply lsegf_lsegf. }
+  eapply derives_trans.
+  2: eauto.
+  entailer!.
+  unff lsegf.
+  Exists ith_tail_fs1_ptr_new ith_format_fs1_ptr_new fs1_sigma_new fs1_sigma_pt_new.
+  entailer!.
+  unfold concrete_mformat.
+  entailer!. } 
+do 2 forward.
+{ entailer!; unnw; desf. }
+forward_call(empty_sigma, empty_sigma_pt, gv).
+forward.
+forward_call(t_format, empty_ptr, gv).
+{ prove_ptr; entailer!. }
+forward.
+forward_call(t_flist, gv).
+Intros new_result_tail_ptr.
+do 2 forward.
+dest_ptr new_result_tail_ptr.
+forward_call(gv).
+Intros new_empty_ptr.
+do 6 forward.
+Exists (filter (fun G : t => (height G <=? Z.to_nat h)%nat)
+        (aboveDoc (Z.to_nat w) fs1 (sublist 0 i fs2)) ++
+        filter (fun G : t => (height G <=? Z.to_nat h)%nat)
+        (aboveDoc (Z.to_nat w) (sublist 0 (j + 1) fs1) [Znth i fs2])) new_result_tail_ptr.
+entailer!.
+2: { 
+  unfold mformat.
+  Intros sigma0 sigma_pt0.
+  unff listrepf.
+  Exists nullval new_empty_ptr sigma0 sigma_pt0.
+  unfold concrete_mformat.
+  entailer!.
+  remember ((filter (fun G : t => (height G <=? Z.to_nat h)%nat) (aboveDoc (Z.to_nat w) fs1 (sublist 0 i fs2)))) as part1.
+  remember (filter (fun G : t => (height G <=? Z.to_nat h)%nat) (aboveDoc (Z.to_nat w) (sublist 0 j fs1) [Znth i fs2])) as part2.
+  remember (filter (fun G : t => (height G <=? Z.to_nat h)%nat) (aboveDoc (Z.to_nat w) (sublist 0 (j + 1) fs1) [Znth i fs2])) as part3.
+  remember (filter (fun G : t => (height G <=? Z.to_nat h)%nat) (aboveDoc (Z.to_nat w) [Znth j fs1] [Znth i fs2])) as part4.
+  assert (part1 ++ part3 = (part1 ++ part2) ++ part4) as K.
+  { rewrite <- app_assoc.
+    apply app_inv_head_iff.
+    vauto.
+    replace (sublist 0 (j + 1) fs1) with (sublist 0 j fs1 ++ [Znth j fs1]) by list_solve.
+    rewrite <- above_doc_app_l.
+    rewrite filter_app; vauto. }
+  rewrite K.
+  assert(
+    listrepf (sublist j (Zlength fs1) fs1) head_ptr2 w h
+    * listrepf (sublist i (Zlength fs2) fs2) head_ptr w h
+    * lsegf (part1 ++ part2) result_ptr result_tail_ptr_new w h
+    * lsegf part4 result_tail_ptr_new new_result_tail_ptr w h |--
+    listrepf (sublist j (Zlength fs1) fs1) head_ptr2 w h
+      * listrepf (sublist i (Zlength fs2) fs2) head_ptr w h
+      * lsegf ((part1 ++ part2) ++ part4) result_ptr new_result_tail_ptr w h
+  ) as FF.
+  { entailer!.
+    apply lsegf_lsegf. }
+  eapply derives_trans.
+  2: eauto.
+  entailer!.
+  unfold FormatTrivial.aboveDoc.
+  unfold FormatTrivial.cross_general.
+  rewrite map_cons.
+  rewrite map_nil.
+  rewrite map_cons.
+  rewrite map_nil.
+  rewrite concat_cons.
+  rewrite concat_nil.
+  autorewrite with sublist.
+  unfold filter.
+  desf;
+  assert (
+    (total_width (add_above (Znth j fs1) (Znth i fs2)) <= Z.to_nat w)%nat /\
+      (height (add_above (Znth j fs1) (Znth i fs2)) <= Z.to_nat h)%nat
+  ) as GG by auto; desf.
+  unff lsegf.
+  Exists new_result_tail_ptr result_format_ptr result_sigma result_sigma_pt.
+  entailer!.
+  { unfold good_format; split; vauto. }
+  unfold concrete_mformat; entailer!.
+  assert (
+    listrepf (sublist j (Zlength fs1) fs1) head_ptr2 w h
+    * lsegf [Znth i fs2] head_ptr ith_tail_fs2_ptr w h
+    * listrepf (sublist (i + 1) (Zlength fs2) fs2) ith_tail_fs2_ptr w h |--
+    listrepf (sublist j (Zlength fs1) fs1) head_ptr2 w h
+    * listrepf (sublist i (Zlength fs2) fs2) head_ptr w h
+  ) as KK.
+  { entailer!.
+    replace (sublist i (Zlength fs2) fs2) 
+      with ([Znth i fs2] ++ sublist (i + 1) (Zlength fs2) fs2) by list_solve.
+    apply lsegf_listf. }
+  eapply derives_trans.
+  2: eauto.
+  entailer!.
+  unff lsegf.
+  Exists ith_tail_fs2_ptr ith_format_fs2_ptr fs2_sigma fs2_sigma_pt.
+  unfold concrete_mformat.
+  entailer!.
+  assert(
+    lsegf [Znth j fs1] head_ptr2 ith_tail_fs1_ptr w h
+    * listrepf (sublist (j + 1) (Zlength fs1) fs1) ith_tail_fs1_ptr w h |--
+    listrepf (sublist j (Zlength fs1) fs1) head_ptr2 w h
+  ) as KKK.
+  { replace (sublist j (Zlength fs1) fs1) with
+      ([Znth j fs1] ++ sublist (j + 1) (Zlength fs1) fs1) by list_solve.
+    apply lsegf_listf. }
+  eapply derives_trans.
+  2: eauto.
+  entailer!.
+  unff lsegf.
+  Exists ith_tail_fs1_ptr ith_format_fs1_ptr fs1_sigma fs1_sigma_pt.
+  unfold concrete_mformat.
+  entailer!. }
+autorewrite with sublist norm.
+desf.
+remember (filter (fun G : t => (height G <=? Z.to_nat h)%nat) (aboveDoc (Z.to_nat w) (sublist 0 j fs1) [Znth i fs2])) as part2.
+remember ((filter (fun G : t => (height G <=? Z.to_nat h)%nat) (aboveDoc (Z.to_nat w) fs1 (sublist 0 i fs2)))) as part1.
+remember (filter (fun G : t => (height G <=? Z.to_nat h)%nat) (aboveDoc (Z.to_nat w) (sublist 0 (j + 1) fs1) [Znth i fs2])) as part3.
+remember (filter (fun G : t => (height G <=? Z.to_nat h)%nat) (aboveDoc (Z.to_nat w) [Znth j fs1] [Znth i fs2])) as part4.
+assert (part3 = part2 ++ part4) as K.
+{ vauto.
+  replace (sublist 0 (j + 1) fs1) with (sublist 0 j fs1 ++ [Znth j fs1]) by list_solve.
+  rewrite <- above_doc_app_l.
+  rewrite filter_app; vauto. }
+rewrite K.
+rewrite Zlength_app.
+enough (Zlength part4 = 1) as KK. 
+{ rewrite KK.
+  assert(Zlength part1 + Zlength part2 + 1 > 0) as FF.
+  { list_solve. }
+  assert (0 <? Zlength part1 + (Zlength part2 + 1) = true) as GG.
+  { lia. }
+  rewrite GG.
+  list_solve. }
+vauto.
+unfold aboveDoc.
+unfold cross_general.
+rewrite map_cons.
+rewrite map_nil.
+rewrite map_cons.
+rewrite map_nil.
+rewrite concat_cons.
+rewrite concat_nil.
+autorewrite with sublist.
+unfold filter.
+desf;
+assert (
+  (total_width (add_above (Znth j fs1) (Znth i fs2)) <= Z.to_nat w)%nat /\
+    (height (add_above (Znth j fs1) (Znth i fs2)) <= Z.to_nat h)%nat
 ) as GG by auto; desf.
 Qed.
